refactor(Normal Modal): Refactor lemmata and notations (#26)
* refactor: consistency lemmata for Hibert style deduction

* refactor: Hilbertean deducible lemmata

* feat: hilbert dt lemma

* refactor(Normal Modal): remove some deprecated

* refactor(Normal Modal): remove more deprecated

* refactor(Normal Modal): remove box dia lemmata `Theory` and `Context`

* feat(Normal Modal): semantics lemmata and explicit soundness proof

* refactor(Normal Modal): satisfy notation

* feat(Normal Modal): FrameClassDefinability

* refactor(Normal Modal): unsatisfies

* fix(Normal Modal): fixed by review

Logic/Logic/HilbertStyle2.lean
@@ -15,11 +15,25 @@ section
 
 variable (Bew : Set F → F → Type*)
 
+class HasModusPonens where
+  modus_ponens {Γ₁ Γ₂ p q} : (Bew Γ₁ (p ⟶ q)) → (Bew Γ₂ p) → (Bew (Γ₁ ∪ Γ₂) q)
+
+section
+
+variable {Bew : Set F → F → Type*} [HasModusPonens Bew]
+
+abbrev modus_ponens {Γ₁ Γ₂ p q} (d₁ : Bew Γ₁ (p ⟶ q)) (d₂ : Bew Γ₂ p) : Bew (Γ₁ ∪ Γ₂) q := HasModusPonens.modus_ponens d₁ d₂
+infixr:90 "⨀" => modus_ponens
+
+def modus_ponens' {Γ p q} (d₁ : Bew Γ (p ⟶ q)) (d₂ : Bew Γ p) : Bew Γ q := by simpa using d₁ ⨀ d₂
+infixr:90 "⨀" => modus_ponens'
+
+end
+
 /--
   Minimal Propositional Logic.
 -/
-class Minimal [NegDefinition F] extends Deduction Bew where
-  modus_ponens {Γ₁ Γ₂ : Set F} {p q : F} : (Bew Γ₁ (p ⟶ q)) → (Bew Γ₂ p) → (Bew (Γ₁ ∪ Γ₂) q)
+class Minimal [NegDefinition F] extends Deduction Bew, HasModusPonens Bew where
   verum        (Γ : Set F)             : Bew Γ ⊤
   imply₁       (Γ : Set F) (p q : F)   : Bew Γ (p ⟶ (q ⟶ p))
   imply₂       (Γ : Set F) (p q r : F) : Bew Γ ((p ⟶ q ⟶ r) ⟶ (p ⟶ q) ⟶ p ⟶ r)
@@ -88,17 +102,11 @@ end
 
 open Deduction Minimal HasDT Intuitionistic Classical HasDNE
 
-infixr:90 " ⨀ " => modus_ponens
-
-variable {Bew : Set F → F → Type*} (Γ : Set F) (p q r : F)
+variable {Bew : Set F → F → Type u} (Γ : Set F) (p q r : F)
 
 section Minimal
 
 variable [hM : Minimal Bew] [hDT : HasDT Bew] [hEFQ : HasEFQ Bew]
-
-def modus_ponens' {Γ p q} (d₁ : Bew Γ (p ⟶ q)) (d₂ : Bew Γ p) : Bew Γ q := by simpa using d₁ ⨀ d₂
-
-infixr:90 " ⨀ " => modus_ponens'
 
 abbrev efq := hEFQ.efq
 
@@ -139,6 +147,10 @@ def disj₂' {Γ p q} (d : Bew Γ q) : Bew Γ (p ⋎ q) := (disj₂ _ _ _ ⨀ d)
 abbrev disj₃ := hM.disj₃
 
 def disj₃' {Γ p q r} (d₁ : Bew Γ (p ⟶ r)) (d₂ : Bew Γ (q ⟶ r)) (d₃ : Bew Γ (p ⋎ q)) : Bew Γ r := (((disj₃ _ _ _ _) ⨀ d₁) ⨀ d₂) ⨀ d₃
+
+def disj_symm' {Γ p q} : Bew Γ (p ⋎ q) → Bew Γ (q ⋎ p) := by
+  intro h;
+  exact disj₃' (disj₂ _ _ _) (disj₁ _ _ _) h;
 
 def iff_mp' {Γ p q} (d : Bew Γ (p ⟷ q)) : Bew Γ (p ⟶ q) := by
   simp [LogicSymbol.iff] at d;
@@ -193,6 +205,47 @@ def neg_iff' {Γ p q} (d : Bew Γ (p ⟷ q)) : Bew Γ (~p ⟷ ~q) := by
   . apply contra₀';
     apply iff_mp' d
 
+def trans' {Γ p q r} (h₁ : Bew Γ (p ⟶ q)) (h₂ : Bew Γ (q ⟶ r)) : Bew Γ (p ⟶ r) := by
+  apply dtr;
+  have : Bew (insert p Γ) p := axm (by simp);
+  have : Bew (insert p Γ) q := modus_ponens' (weakening' (by simp) h₁) this;
+  have : Bew (insert p Γ) r := modus_ponens' (weakening' (by simp) h₂) this;
+  exact this
+
+def assoc_left' {Γ p q r} (h : Bew Γ ((p ⋏ q) ⋏ r)) : Bew Γ (p ⋏ (q ⋏ r)) := by
+  have dpq := conj₁' h;
+  have dp := conj₁' dpq;
+  have dq := conj₂' dpq;
+  have dr := conj₂' h;
+  exact conj₃' dp (conj₃' dq dr)
+
+def assoc_left (Γ p q r) : Bew Γ ((p ⋏ q) ⋏ r ⟶ p ⋏ (q ⋏ r)) := by
+  apply dtr;
+  exact assoc_left' (axm (by simp))
+
+def assoc_right' {Γ p q r} (h : Bew Γ (p ⋏ (q ⋏ r))) : Bew Γ ((p ⋏ q) ⋏ r) := by
+  have dp := conj₁' h;
+  have dqr := conj₂' h;
+  have dq := conj₁' dqr;
+  have dr := conj₂' dqr;
+  exact conj₃' (conj₃' dp dq) dr
+
+def assoc_right (Γ p q r) : Bew Γ (p ⋏ (q ⋏ r) ⟶ (p ⋏ q) ⋏ r) := by
+  apply dtr;
+  exact assoc_right' (axm (by simp))
+
+def assoc (Γ p q r) : Bew Γ ((p ⋏ q) ⋏ r ⟷ p ⋏ (q ⋏ r)) := iff_intro (by apply assoc_left) (by apply assoc_right)
+
+def conj_symm' {Γ p q} : Bew Γ (p ⋏ q) → Bew Γ (q ⋏ p) := by
+  intro h;
+  exact conj₃' (conj₂' h) (conj₁' h);
+
+def conj_symm (Γ p q) : Bew Γ ((p ⋏ q) ⟶ (q ⋏ p)) := by
+  apply dtr;
+  exact conj_symm' (axm (by simp))
+
+def conj_symm_iff (Γ p q) : Bew Γ ((p ⋏ q) ⟷ (q ⋏ p)) := iff_intro (by apply conj_symm) (by apply conj_symm)
+
 end Minimal
 
 section Classical
@@ -219,6 +272,178 @@ instance : HasLEM Bew where
   lem Γ p := by sorry;
 
 end Classical
+
+section
+
+variable [LogicSymbol F] [NegDefinition F]
+variable (Bew : Set F → F → Type u) [hd : Deduction Bew] [HasModusPonens Bew] [HasDT Bew] [Minimal Bew] [Classical Bew]
+
+local infix:20 " ⊢ " => Bew
+
+variable (Γ : Set F) (p : F)
+
+@[simp] def Deducible := Nonempty (Bew Γ p)
+@[simp] def Undeducible := ¬(Deducible Bew Γ p)
+
+section Deducible
+
+variable {Bew : Set F → F → Type u} [Deduction Bew]
+variable [HasDT Bew] [HasModusPonens Bew] [Minimal Bew] [Classical Bew]
+
+local infix:20 "⊢!" => Deducible Bew
+local infix:20 "⊬!" => Undeducible Bew
+
+lemma axm! {Γ : Set F} {f : F} (h : f ∈ Γ) : Γ ⊢! f := ⟨axm h⟩
+
+lemma weakening! {Γ Δ : Set F} {p : F} (h : Γ ⊆ Δ) (d : Γ ⊢! p) : Δ ⊢! p := ⟨weakening' h d.some⟩
+
+lemma modus_ponens! {Γ₁ Γ₂ : Set F} {p q : F} (d₁ : Γ₁ ⊢! (p ⟶ q)) (d₂ : Γ₂ ⊢! p) : Deducible Bew (Γ₁ ∪ Γ₂) q := ⟨d₁.some ⨀ d₂.some⟩
+lemma modus_ponens'! {Γ : Set F} {p q : F} (d₁ : Γ ⊢! (p ⟶ q)) (d₂ : Γ ⊢! p) : Γ ⊢! q := by simpa using modus_ponens! d₁ d₂
+
+lemma verum! (Γ : Set F) : Γ ⊢! ⊤ := ⟨verum Γ⟩
+
+lemma imply₁! (Γ : Set F) (p q : F) : Γ ⊢! (p ⟶ q ⟶ p) := ⟨imply₁ Γ p q⟩
+lemma imply₁'! {Γ : Set F} {p q : F} (d : Γ ⊢! p) : Γ ⊢! (q ⟶ p) := ⟨imply₁' d.some⟩
+
+lemma imply₂! (Γ : Set F) (p q r : F) : Γ ⊢! ((p ⟶ q ⟶ r) ⟶ (p ⟶ q) ⟶ p ⟶ r) := ⟨imply₂ Γ p q r⟩
+lemma imply₂'! {Γ : Set F} {p q r : F} (d₁ : Γ ⊢! (p ⟶ q ⟶ r)) (d₂ : Γ ⊢! (p ⟶ q)) (d₃ : Γ ⊢! p) : Γ ⊢! r := ⟨imply₂' d₁.some d₂.some d₃.some⟩
+
+lemma conj₁! (Γ : Set F) (p q : F) : Γ ⊢! (p ⋏ q ⟶ p) := ⟨conj₁ Γ p q⟩
+lemma conj₁'! {Γ : Set F} {p q : F} (d : Γ ⊢! (p ⋏ q)) : Γ ⊢! p := ⟨conj₁' d.some⟩
+
+lemma conj₂! (Γ : Set F) (p q : F) : Γ ⊢! (p ⋏ q ⟶ q) := ⟨conj₂ Γ p q⟩
+lemma conj₂'! {Γ : Set F} {p q : F} (d : Γ ⊢! (p ⋏ q)) : Γ ⊢! q := ⟨conj₂' d.some⟩
+
+lemma conj₃! (Γ : Set F) (p q : F) : Γ ⊢! (p ⟶ q ⟶ p ⋏ q) := ⟨conj₃ Γ p q⟩
+lemma conj₃'! {Γ : Set F} {p q : F} (d₁ : Γ ⊢! p) (d₂: Γ ⊢! q) : Γ ⊢! (p ⋏ q) := ⟨conj₃' d₁.some d₂.some⟩
+
+lemma conj_symm'! {Γ : Set F} {p q : F} (d : Γ ⊢! (p ⋏ q)) : Γ ⊢! (q ⋏ p) := ⟨conj_symm' d.some⟩
+
+lemma disj₁! (Γ : Set F) (p q : F) : Γ ⊢! (p ⟶ p ⋎ q) := ⟨disj₁ Γ p q⟩
+lemma disj₁'! {Γ : Set F} {p q : F} (d : Γ ⊢! p) : Γ ⊢! (p ⋎ q) := ⟨disj₁' d.some⟩
+
+lemma disj₂! (Γ : Set F) (p q : F) : Γ ⊢! (q ⟶ p ⋎ q) := ⟨disj₂ Γ p q⟩
+lemma disj₂'! {Γ : Set F} {p q : F} (d : Γ ⊢! q) : Γ ⊢! (p ⋎ q) := ⟨disj₂' d.some⟩
+
+lemma disj₃! (Γ : Set F) (p q r : F) : Γ ⊢! ((p ⟶ r) ⟶ (q ⟶ r) ⟶ (p ⋎ q) ⟶ r) := ⟨disj₃ Γ p q r⟩
+lemma disj₃'! {Γ : Set F} {p q r : F} (d₁ : Γ ⊢! (p ⟶ r)) (d₂ : Γ ⊢! (q ⟶ r)) (d₃ : Γ ⊢! (p ⋎ q)) : Γ ⊢! r := ⟨disj₃' d₁.some d₂.some d₃.some⟩
+
+lemma disj_symm'! {Γ : Set F} {p q : F} (d : Γ ⊢! (p ⋎ q)) : Γ ⊢! (q ⋎ p) := ⟨disj_symm' d.some⟩
+
+lemma efq! [HasEFQ Bew] (Γ : Set F) (p : F) : Γ ⊢! (⊥ ⟶ p) := ⟨efq Γ p⟩
+lemma efq'! [HasEFQ Bew] {Γ : Set F} {p} (d : Γ ⊢! ⊥) : Γ ⊢! p := ⟨efq' d.some⟩
+
+lemma dni! (Γ : Set F) (p : F) : Γ ⊢! (p ⟶ ~~p) := ⟨dni Γ p⟩
+lemma dni'! {Γ : Set F} {p} (d : Γ ⊢! p) : Γ ⊢! (~~p) := ⟨dni' d.some⟩
+
+lemma dne! [HasDNE Bew] (Γ : Set F) (p : F) : Γ ⊢! (~~p ⟶ p) := ⟨dne Γ p⟩
+lemma dne'! [HasDNE Bew] {Γ : Set F} {p} (d : Γ ⊢! (~~p)) : Γ ⊢! p := ⟨dne' d.some⟩
+
+lemma equiv_dn! (Γ : Set F) (p : F) : Γ ⊢! (p ⟷ ~~p) := ⟨equiv_dn Γ p⟩
+
+lemma iff_intro! {Γ : Set F} {p q : F} (dpq : Γ ⊢! (p ⟶ q)) (dqp : Γ ⊢! (q ⟶ p)) : Γ ⊢! (p ⟷ q) := ⟨iff_intro dpq.some dqp.some⟩
+
+lemma iff_symm'! {Γ : Set F} {p q : F} (d : Γ ⊢! (p ⟷ q)) : Γ ⊢! (q ⟷ p) := ⟨iff_symm' d.some⟩
+
+lemma iff_mp'! {Γ : Set F} {p q : F} (d : Γ ⊢! (p ⟷ q)) : Γ ⊢! (p ⟶ q) := ⟨iff_mp' d.some⟩
+lemma iff_mpr'! {Γ : Set F} {p q : F} (d : Γ ⊢! (p ⟷ q)) : Γ ⊢! (q ⟶ p) := ⟨iff_mpr' d.some⟩
+
+lemma iff_left'! {Γ : Set F} {p q : F} (dpq : Γ ⊢! (p ⟷ q)) (dq : Γ ⊢! q) : Γ ⊢! p := ⟨iff_left' dpq.some dq.some⟩
+lemma iff_right'! {Γ : Set F} {p q : F} (dpq : Γ ⊢! (p ⟷ q)) (dp : Γ ⊢! p) : Γ ⊢! q := ⟨iff_right' dpq.some dp.some⟩
+
+lemma iff_def! {Γ : Set F} {p q : F} : (Γ ⊢! (p ⟷ q)) ↔ (Γ ⊢! (p ⟶ q)) ∧ (Γ ⊢! (q ⟶ p)) := by
+  constructor;
+  . intro h; exact ⟨iff_mp'! h, iff_mpr'! h⟩
+  . intro h; exact iff_intro! h.1 h.2
+
+lemma neg_iff'! {Γ : Set F} {p q : F} (d : Γ ⊢! (p ⟷ q)) : Γ ⊢! (~p ⟷ ~q) := ⟨neg_iff' d.some⟩
+
+lemma contra₀'! {Γ : Set F} {p q : F} (d : Γ ⊢! (p ⟶ q)) : Γ ⊢! (~q ⟶ ~p) := ⟨contra₀' d.some⟩
+
+lemma dtr! {Γ : Set F} {p q : F} (d : (insert p Γ) ⊢! q) : Γ ⊢! (p ⟶ q) := ⟨dtr d.some⟩
+lemma dtr_not! {Γ : Set F} {p q : F} : (Γ ⊬! (p ⟶ q)) → ((insert p Γ) ⊬! q) := by
+  contrapose;
+  simp;
+  intro d;
+  exact ⟨dtr d⟩
+
+lemma dtl! {Γ : Set F} {p q : F} (d : Γ ⊢! (p ⟶ q)) : (insert p Γ) ⊢! q := ⟨dtl d.some⟩
+lemma dtl_not! {Γ : Set F} {p q : F} : ((insert p Γ) ⊬! q) → (Γ ⊬! (p ⟶ q)) := by
+  contrapose;
+  simp;
+  intro d;
+  exact ⟨dtl d⟩
+
+end Deducible
+
+section Consistency
+
+local infix:20 "⊢!" => Deducible Bew
+local infix:20 "⊬!" => Undeducible Bew
+
+@[simp] def Inconsistent := Γ ⊢! ⊥
+@[simp] def Consistent := Γ ⊬! ⊥
+
+lemma consistent_iff_undeducible_falsum : Consistent Bew Γ ↔ (Γ ⊬! ⊥) := Iff.rfl
+
+lemma consistent_no_falsum {Γ} (h : Consistent Bew Γ) : ⊥ ∉ Γ := by
+  by_contra hC;
+  exact h ⟨hd.axm hC⟩
+
+lemma consistent_of_subset {Γ Δ : Set F} (h : Γ ⊆ Δ) (hConsis : Consistent Bew Δ) : Consistent Bew Γ := by
+  intro hD;
+  exact hConsis ⟨hd.weakening' h hD.some⟩;
+
+lemma consistent_of_insert {p} (hConsis : Consistent Bew (insert p Γ)) : Consistent Bew Γ := consistent_of_subset Bew (by simp) hConsis
+
+lemma consistent_no_falsum_subset {Γ Δ} (hConsis : Consistent Bew Γ) (hΔ : Δ ⊆ Γ) : ⊥ ∉ Δ := consistent_no_falsum Bew $ consistent_of_subset Bew hΔ hConsis
+
+lemma consistent_subset_undeducible_falsum {Γ Δ} (hConsis : Consistent Bew Γ) (hΔ : Δ ⊆ Γ) : (Δ ⊬! ⊥) := by
+  by_contra hC;
+  simp_all [Consistent, Undeducible, Deducible];
+  exact hConsis.false $ hd.weakening' hΔ hC.some;
+
+lemma consistent_neither_undeducible {Γ : Set F} (hConsis : Consistent Bew Γ) (p) : (Γ ⊬! p) ∨ (Γ ⊬! ~p) := by
+  by_contra hC; simp only [not_or] at hC;
+  have h₁ : Γ ⊢! p  := by simpa using hC.1;
+  have h₂ : Γ ⊢! p ⟶ ⊥ := by simpa using hC.2;
+  exact hConsis $ modus_ponens'! h₂ h₁;
+
+lemma inconsistent_of_deduction {Γ : Set F} (d : Γ ⊢ ⊥) : Inconsistent Bew Γ := ⟨d⟩
+
+lemma inconsistent_of_deducible {Γ : Set F} (d : Γ ⊢! ⊥) : Inconsistent Bew Γ := by simpa [Inconsistent];
+
+lemma inconsistent_insert_falsum : Inconsistent Bew (insert ⊥ Γ) := ⟨hd.axm (by simp)⟩
+
+lemma inconsistent_insert {Γ p} (h : Inconsistent Bew (insert p Γ)) : (∃ Δ, (Δ ⊆ Γ) ∧ ((insert p Δ) ⊢! ⊥)) := by
+  existsi Γ;
+  constructor;
+  . rfl;
+  . exact h;
+
+/--
+  **This lemma require classical logic.**
+-/
+lemma inconsistent_iff_insert_neg {Γ p} : Inconsistent Bew (insert (~p) Γ) ↔ (Γ ⊢! p) := by
+  constructor;
+  . intro h;
+    have : Γ ⊢ ~~p := by simpa using (dtr h.some);
+    exact ⟨(dne' this)⟩
+  . intro h;
+    have : Γ ⊢ ((p ⟶ ⊥) ⟶ ⊥) := by simpa using dni' h.some
+    exact ⟨by simpa using (dtl this)⟩;
+
+lemma consistent_iff_insert_neg {Γ p} : Consistent Bew (insert (~p) Γ) ↔ (Γ ⊬! p) := (inconsistent_iff_insert_neg Bew).not
+
+lemma consistent_either {Γ : Set F} (hConsis : Consistent Bew Γ) (p) : (Consistent Bew (insert p Γ)) ∨ (Consistent Bew (insert (~p) Γ)) := by
+  by_contra hC; simp [not_or, Consistent] at hC;
+  have ⟨Δ₁, hΔ₁, ⟨dΔ₁⟩⟩ := inconsistent_insert Bew hC.1;
+  have ⟨Δ₂, hΔ₂, ⟨dΔ₂⟩⟩ := inconsistent_insert Bew hC.2;
+  exact consistent_subset_undeducible_falsum _ hConsis (by aesop) ⟨(dtr dΔ₂) ⨀ (dtr dΔ₁)⟩;
+
+end Consistency
+
+end
 
 end Hilbert
 
