Logic/Modal/Normal/LogicSymbol.lean
@@ -13,7 +13,9 @@ class ModalLogicSymbol (α : Sort _) extends LogicSymbol α, Box α, Dia α
 prefix:74 "□" => Box.box
 prefix:74 "◇" => Dia.dia
 
-attribute [match_pattern] Box.box Dia.dia
+attribute [match_pattern]
+  Box.box
+  Dia.dia
 
 /-- Diamond(`◇`) defined by Box(`□`) -/
 class ModalDuality (F : Type*) [ModalLogicSymbol F] where
@@ -28,3 +30,87 @@ class ModalDuality' (F : Type*) [ModalLogicSymbol F] where
 attribute [simp] ModalDuality'.box
 
 end LO.Modal.Normal
+
+
+namespace Set
+
+open LO.Modal.Normal
+
+variable [ModalLogicSymbol α]
+
+def box (s : Set α) : Set α := Box.box '' s
+
+@[simp]
+lemma box_empty : (∅ : Set α).box = ∅ := by simp [Set.box]
+
+lemma box_subset {s t : Set α} (h : s ⊆ t) : s.box ⊆ t.box := by simp_all [Set.subset_def, box]; aesop;
+
+lemma box_union {s t : Set α} : (s ∪ t).box = s.box ∪ t.box := by simp_all [Set.image_union, box];
+
+@[simp]
+lemma box_mem_intro {s : Set α} {a : α} : a ∈ s → □a ∈ s.box := by simp_all [box]; aesop;
+
+lemma box_mem_iff {s : Set α} {p : α} : p ∈ s.box ↔ (∃ q ∈ s, □q = p) := by simp_all [Set.mem_image, box]
+
+
+def dia (s : Set α) : Set α := Dia.dia '' s
+
+@[simp]
+lemma dia_empty : (∅ : Set α).dia = ∅ := by simp [Set.dia]
+
+lemma dia_subset {s t : Set α} (h : s ⊆ t) : s.dia ⊆ t.dia := by simp_all [Set.subset_def, dia]; aesop;
+
+lemma dia_union {s t : Set α} : (s ∪ t).dia = s.dia ∪ t.dia := by simp_all [Set.image_union, dia];
+
+@[simp]
+lemma dia_mem_intro {s : Set α} {a : α} : a ∈ s → ◇a ∈ s.dia := by simp_all [dia]; aesop;
+
+lemma dia_mem_iff {s : Set α} {p : α} : p ∈ s.dia ↔ (∃ q ∈ s, ◇q = p) := by simp_all [Set.mem_image, dia]
+
+
+def prebox (s : Set α) := Box.box ⁻¹' s
+
+@[simp]
+lemma prebox_box_eq (s : Set α) : s.prebox.box = { □p | (p : α) (_ : □p ∈ s) } := by aesop;
+
+@[simp]
+lemma prebox_box_subset {s : Set α} : s.prebox.box ⊆ s := by simp [Set.subset_def];
+
+lemma prebox_subset {s t : Set α} (h : s ⊆ t) : s.prebox ⊆ t.prebox := by simp_all [Set.subset_def, prebox];
+
+
+def predia (s : Set α) := Dia.dia ⁻¹' s
+
+@[simp]
+lemma predia_dia_eq (s : Set α) : s.predia.dia = { ◇p | (p : α) (_ : ◇p ∈ s) } := by aesop;
+
+@[simp]
+lemma predia_dia_subset {s : Set α} : s.predia.dia ⊆ s := by simp [Set.subset_def];
+
+lemma predia_subset {s t : Set α} (h : s ⊆ t) : s.predia ⊆ t.predia := by simp_all [Set.subset_def, predia];
+
+end Set
+
+
+namespace Finset
+
+open LO.Modal.Normal
+
+variable [ModalLogicSymbol α] [DecidableEq α]
+
+def box (s : Finset α) : Finset α := s.image Box.box
+
+lemma box_union {s t : Finset α} : ((s ∪ t).box : Finset α) = (s.box ∪ t.box : Finset α) := by simp_all [Finset.image_union, box];
+
+@[simp]
+lemma box_coe {s : Finset α} : (↑s : Set α).box = ↑(s.box) := by simp only [Set.box, Finset.box, Finset.coe_image];
+
+
+def dia (s : Finset α) : Finset α := s.image Dia.dia
+
+lemma dia_union {s t : Finset α} : ((s ∪ t).dia : Finset α) = (s.dia ∪ t.dia : Finset α) := by simp_all [Finset.image_union, dia];
+
+@[simp]
+lemma dia_coe {s : Finset α} :(↑s : Set α).dia = ↑(s.dia) := by simp only [Set.dia, Finset.dia, Finset.coe_image];
+
+end Finset
