Logic/Modal/Normal/Semantics.lean
@@ -25,35 +25,40 @@ def Satisfies (M : Model α β) (w : α) : Formula β → Prop
   | imp p q => ¬(p.Satisfies M w) ∨ (q.Satisfies M w)
   | box p   => ∀w', M.frame w w' → p.Satisfies M w'
 
-notation "⊧ᴹ[" M "," w "] " p => Satisfies M w p
+notation w " ⊩ᴹ[" M "] " p => Satisfies M w p
+
+@[simp]
+abbrev Unsatisfies (M : Model α β) (w : α) (p : Formula β) := ¬(w ⊩ᴹ[M] p)
+notation w " ⊮ᴹ[" M "] " p => Unsatisfies M w p
 
 namespace Satisfies
 
 variable {M : Model α β}
 
-@[simp] lemma atom_def : (⊧ᴹ[M, w] atom a) ↔ a ∈ M.val w := by simp [Satisfies];
+@[simp] lemma atom_def : (w ⊩ᴹ[M] atom a) ↔ a ∈ M.val w := by simp [Satisfies];
 
-@[simp] lemma top_def : (⊧ᴹ[M, w] ⊤) := by simp [Satisfies];
+@[simp] lemma top_def : (w ⊩ᴹ[M] ⊤) := by simp [Satisfies];
 
-@[simp] lemma bot_def : (⊧ᴹ[M, w] ⊥) ↔ False := by simp [Satisfies];
+@[simp] lemma bot_def : (w ⊩ᴹ[M] ⊥) ↔ False := by simp [Satisfies];
 
-@[simp] lemma and_def : (⊧ᴹ[M, w] p ⋏ q) ↔ (⊧ᴹ[M, w] p) ∧ (⊧ᴹ[M, w] q) := by simp [Satisfies];
+@[simp] lemma and_def : (w ⊩ᴹ[M] p ⋏ q) ↔ (w ⊩ᴹ[M] p) ∧ (w ⊩ᴹ[M] q) := by simp [Satisfies];
 
-@[simp] lemma or_def : (⊧ᴹ[M, w] p ⋎ q) ↔ (⊧ᴹ[M, w] p) ∨ (⊧ᴹ[M, w] q) := by simp [Satisfies];
+@[simp] lemma or_def : (w ⊩ᴹ[M] p ⋎ q) ↔ (w ⊩ᴹ[M] p) ∨ (w ⊩ᴹ[M] q) := by simp [Satisfies];
 
-lemma imp_def : (⊧ᴹ[M, w] p ⟶ q) ↔ ¬(⊧ᴹ[M, w] p) ∨ (⊧ᴹ[M, w] q) := by simp [Satisfies];
-@[simp] lemma imp_def' : (⊧ᴹ[M, w] p ⟶ q) ↔ (⊧ᴹ[M, w] p) → (⊧ᴹ[M, w] q) := by simp [Satisfies, imp_iff_not_or];
+lemma imp_def : (w ⊩ᴹ[M] p ⟶ q) ↔ (w ⊮ᴹ[M] p) ∨ (w ⊩ᴹ[M] q) := by simp [Satisfies];
+@[simp] lemma imp_def' : (w ⊩ᴹ[M] p ⟶ q) ↔ (w ⊩ᴹ[M] p) → (w ⊩ᴹ[M] q) := by simp [Satisfies, imp_iff_not_or];
 
-@[simp] lemma box_def : (⊧ᴹ[M, w] □p) ↔ (∀w', M.frame w w' → (⊧ᴹ[M, w'] p)) := by simp [Satisfies];
-@[simp] lemma dia_def : (⊧ᴹ[M, w] ◇p) ↔ (∃w', M.frame w w' ∧ (⊧ᴹ[M, w'] p)) := by simp [Satisfies];
+@[simp] lemma box_def : (w ⊩ᴹ[M] □p) ↔ (∀w', M.frame w w' → (w' ⊩ᴹ[M] p)) := by simp [Satisfies];
+@[simp] lemma dia_def : (w ⊩ᴹ[M] ◇p) ↔ (∃w', M.frame w w' ∧ (w' ⊩ᴹ[M] p)) := by simp [Satisfies];
 
-@[simp] lemma neg_def : (⊧ᴹ[M, w] (neg p)) ↔ ¬(⊧ᴹ[M, w] p) := by simp [Satisfies];
-@[simp] lemma neg_def' : (⊧ᴹ[M, w] ~p) ↔ ¬(⊧ᴹ[M, w] p) := by simp [Satisfies];
+@[simp] lemma neg_def : (w ⊩ᴹ[M] (neg p)) ↔ (w ⊮ᴹ[M] p) := by simp [Satisfies];
+@[simp] lemma neg_def' : (w ⊩ᴹ[M] ~p) ↔ (w ⊮ᴹ[M] p) := by simp [Satisfies];
+
+lemma modus_ponens (m₁ : w ⊩ᴹ[M] p ⟶ q) : (w ⊩ᴹ[M] p) → (w ⊩ᴹ[M] q) := by simpa [imp_def'] using m₁;
 
 end Satisfies
 
-
-def Models (M : Model α β) (p : Formula β) := ∀w, (⊧ᴹ[M, w] p)
+def Models (M : Model α β) (p : Formula β) := ∀w, (w ⊩ᴹ[M] p)
 notation "⊧ᴹ[" M "] "  p => Models M p
 
 namespace Models
@@ -72,6 +77,26 @@ lemma modus_ponens : (⊧ᴹ[M] p ⟶ q) → (⊧ᴹ[M] p) → (⊧ᴹ[M] q) := 
 
 lemma necessitation : (⊧ᴹ[M] p) → (⊧ᴹ[M] □p) := by simp_all [Models, Satisfies];
 
+lemma imply₁ : ⊧ᴹ[M] p ⟶ q ⟶ p := by simp_all [Models];
+
+lemma imply₂ : ⊧ᴹ[M] (p ⟶ q ⟶ r) ⟶ (p ⟶ q) ⟶ p ⟶ r := by simp_all [Models];
+
+lemma conj₁ : ⊧ᴹ[M] p ⋏ q ⟶ p := by simp_all [Models];
+
+lemma conj₂ : ⊧ᴹ[M] p ⋏ q ⟶ q := by simp_all [Models];
+
+lemma conj₃ : ⊧ᴹ[M] p ⟶ q ⟶ p ⋏ q := by simp_all [Models];
+
+lemma disj₁ : ⊧ᴹ[M] p ⟶ p ⋎ q := by simp_all [Models];
+
+lemma disj₂ : ⊧ᴹ[M] q ⟶ p ⋎ q := by simp_all [Models];
+
+lemma disj₃ : ⊧ᴹ[M] (p ⟶ r) ⟶ (q ⟶ r) ⟶ p ⋎ q ⟶ r := by simp_all [Models]; aesop;
+
+lemma dne : ⊧ᴹ[M] ~~p ⟶ p := by simp_all [Models];
+
+lemma verum : ⊧ᴹ[M] ⊤ := by simp [Models];
+
 end Models
 
 
@@ -87,15 +112,35 @@ variable {F: Frame α}
 
 lemma modus_ponens : (⊧ᴹ[F] p ⟶ q) → (⊧ᴹ[F] p) → (⊧ᴹ[F] q) := by
   intro h₁ h₂ V;
-  apply Models.modus_ponens (h₁ V) (h₂ V);
+  exact Models.modus_ponens (h₁ V) (h₂ V);
 
 lemma necessitation : (⊧ᴹ[F] p) → (⊧ᴹ[F] □p) := by
   intro h V;
-  apply Models.necessitation (h V);
+  exact Models.necessitation (h V);
+
+lemma verum : ⊧ᴹ[F] (⊤ : Formula β) := by simp only [Frames, Models.verum, forall_const];
+
+lemma imply₁ : ⊧ᴹ[F] p ⟶ q ⟶ p := by simp only [Frames, Models.imply₁, forall_const];
+
+lemma imply₂ : ⊧ᴹ[F] (p ⟶ q ⟶ r) ⟶ (p ⟶ q) ⟶ p ⟶ r := by simp only [Frames, Models.imply₂, forall_const];
+
+lemma conj₁ : ⊧ᴹ[F] p ⋏ q ⟶ p := by simp only [Frames, Models.conj₁, forall_const];
+
+lemma conj₂ : ⊧ᴹ[F] p ⋏ q ⟶ q := by simp only [Frames, Models.conj₂, forall_const];
+
+lemma conj₃ : ⊧ᴹ[F] p ⟶ q ⟶ p ⋏ q := by simp only [Frames, Models.conj₃, forall_const];
+
+lemma disj₁ : ⊧ᴹ[F] p ⟶ p ⋎ q := by simp only [Frames, Models.disj₁, forall_const];
+
+lemma disj₂ : ⊧ᴹ[F] q ⟶ p ⋎ q := by simp only [Frames, Models.disj₂, forall_const];
+
+lemma disj₃ : ⊧ᴹ[F] (p ⟶ r) ⟶ (q ⟶ r) ⟶ p ⋎ q ⟶ r := by simp only [Frames, Models.disj₃, forall_const];
+
+lemma dne : ⊧ᴹ[F] ~~p ⟶ p := by simp only [Frames, Models.dne, forall_const];
 
 end Frames
 
-lemma not_Frames : (∃ V w, ¬(⊧ᴹ[⟨F, V⟩, w] p)) → ¬(⊧ᴹ[F] p) := by
+lemma not_Frames : (∃ V w, (w ⊮ᴹ[⟨F, V⟩] p)) → ¬(⊧ᴹ[F] p) := by
   simp;
   intro V w hw hf;
   exact hw $ hf V w;
@@ -103,9 +148,13 @@ lemma not_Frames : (∃ V w, ¬(⊧ᴹ[⟨F, V⟩, w] p)) → ¬(⊧ᴹ[F] p) :=
 end Formula
 
 
-@[simp]
-def Theory.Satisfies (M : Model α β) (w : α) (Γ : Theory β) := ∀ p ∈ Γ, ⊧ᴹ[M, w] p
-notation "⊧ᴹ[" M "," w "] " Γ => Theory.Satisfies M w Γ
+@[simp] def Theory.Satisfies (M : Model α β) (w : α) (Γ : Theory β) := ∀ p ∈ Γ, w ⊩ᴹ[M] p
+notation w "⊩ᴹ[" M "] " Γ => Theory.Satisfies M w Γ
+
+@[simp] abbrev Theory.Unsatisfies (M : Model α β) (w : α) (Γ : Theory β) := ¬(w ⊩ᴹ[M] Γ)
+notation w "⊮ᴹ[" M "] " Γ => Theory.Unsatisfies M w Γ
+
+variable [DecidableEq β]
 
 @[simp]
 def Theory.Models (M : Model α β) (Γ : Theory β) := ∀ p ∈ Γ, ⊧ᴹ[M] p
@@ -126,11 +175,31 @@ variable {𝔽 : FrameClass α} {p q : Formula β}
 
 lemma modus_ponens : (⊧ᴹ[𝔽] p ⟶ q) → (⊧ᴹ[𝔽] p) → (⊧ᴹ[𝔽] q) := by
   intro h₁ h₂ F hF;
-  apply Frames.modus_ponens (h₁ F hF) (h₂ F hF);
+  exact Frames.modus_ponens (h₁ F hF) (h₂ F hF);
 
 lemma necessitation : (⊧ᴹ[𝔽] p) → (⊧ᴹ[𝔽] □p) := by
   intro h F hF;
-  apply Frames.necessitation (h F hF);
+  exact Frames.necessitation (h F hF);
+
+lemma verum : ⊧ᴹ[𝔽] (⊤ : Formula β) := by simp [FrameClasses, Frames.verum];
+
+lemma imply₁ : ⊧ᴹ[𝔽] p ⟶ q ⟶ p := by simp [FrameClasses, Frames.imply₁];
+
+lemma imply₂ : ⊧ᴹ[𝔽] (p ⟶ q ⟶ r) ⟶ (p ⟶ q) ⟶ p ⟶ r := by simp [FrameClasses, Frames.imply₂];
+
+lemma conj₁ : ⊧ᴹ[𝔽] p ⋏ q ⟶ p := by simp [FrameClasses, Frames.conj₁];
+
+lemma conj₂ : ⊧ᴹ[𝔽] p ⋏ q ⟶ q := by simp [FrameClasses, Frames.conj₂];
+
+lemma conj₃ : ⊧ᴹ[𝔽] p ⟶ q ⟶ p ⋏ q := by simp [FrameClasses, Frames.conj₃];
+
+lemma disj₁ : ⊧ᴹ[𝔽] p ⟶ p ⋎ q := by simp [FrameClasses, Frames.disj₁];
+
+lemma disj₂ : ⊧ᴹ[𝔽] q ⟶ p ⋎ q := by simp [FrameClasses, Frames.disj₂];
+
+lemma disj₃ : ⊧ᴹ[𝔽] (p ⟶ r) ⟶ (q ⟶ r) ⟶ p ⋎ q ⟶ r := by simp [FrameClasses, Frames.disj₃];
+
+lemma dne : ⊧ᴹ[𝔽] ~~p ⟶ p := by simp only [FrameClasses, Frames.dne, implies_true, forall_const];
 
 end Formula.FrameClasses
 
@@ -147,6 +216,10 @@ namespace AxiomSetFrameClass
 lemma union (Λ₁ Λ₂ : AxiomSet β) : (𝔽(Λ₁ ∪ Λ₂) : FrameClass α) = 𝔽(Λ₁) ∩ 𝔽(Λ₂) := by aesop;
 
 lemma triunion (Λ₁ Λ₂ Λ₃ : AxiomSet β) : (𝔽(Λ₁ ∪ Λ₂ ∪ Λ₃) : FrameClass α) = 𝔽(Λ₁) ∩ 𝔽(Λ₂) ∩ 𝔽(Λ₃) := by aesop;
+
+lemma tetraunion (Λ₁ Λ₂ Λ₃ Λ₄ : AxiomSet β) : (𝔽(Λ₁ ∪ Λ₂ ∪ Λ₃ ∪ Λ₄) : FrameClass α) = 𝔽(Λ₁) ∩ 𝔽(Λ₂) ∩ 𝔽(Λ₃) ∩ 𝔽(Λ₄) := by aesop;
+
+lemma pentaunion (Λ₁ Λ₂ Λ₃ Λ₄ Λ₅ : AxiomSet β) : (𝔽(Λ₁ ∪ Λ₂ ∪ Λ₃ ∪ Λ₄ ∪ Λ₅) : FrameClass α) = 𝔽(Λ₁) ∩ 𝔽(Λ₂) ∩ 𝔽(Λ₃) ∩ 𝔽(Λ₄) ∩ 𝔽(Λ₅) := by aesop;
 
 end AxiomSetFrameClass
 
@@ -181,7 +254,7 @@ lemma frames_triunion {F: Frame α} {Γ₁ Γ₂ Γ₃ : Theory β} : (⊧ᴹ[F]
     . exact h.right.left p (by assumption);
     . exact h.right.right p (by assumption);
 
-lemma not_Frames {F: Frame α} {Γ : Theory β} : (∃ V w, ¬(⊧ᴹ[⟨F, V⟩, w] Γ)) → ¬(⊧ᴹ[F] Γ) := by
+lemma not_Frames {F: Frame α} {Γ : Theory β} : (∃ V w, (w ⊮ᴹ[⟨F, V⟩] Γ)) → ¬(⊧ᴹ[F] Γ) := by
   simp [Frames, Satisfies, Formula.Frames, Formula.Models];
   intros V w p hp h;
   existsi p, hp, V, w;
@@ -189,7 +262,7 @@ lemma not_Frames {F: Frame α} {Γ : Theory β} : (∃ V w, ¬(⊧ᴹ[⟨F, V⟩
 
 end Theory
 
-def Formula.FrameConsequence (F : Frame α) (Γ : Theory β) (p : Formula β) := ∀ V w, (⊧ᴹ[⟨F, V⟩, w] Γ) → (⊧ᴹ[⟨F, V⟩, w] p)
+def Formula.FrameConsequence (F : Frame α) (Γ : Theory β) (p : Formula β) := ∀ V w, (w ⊩ᴹ[⟨F, V⟩] Γ) → (w ⊩ᴹ[⟨F, V⟩] p)
 notation Γ " ⊨ᴹ[" F "] " p => Formula.FrameConsequence F Γ p
 notation Γ " ⊭ᴹ[" F "] " p => ¬(Γ ⊨ᴹ[F] p)
 
@@ -216,7 +289,7 @@ lemma modus_ponens' {𝔽 : FrameClass α} {Γ : Theory β} {p : Formula β} : (
 
 end Formula.FrameClassConsequence
 
-def Theory.FrameSatisfiable (F : Frame α) (Γ : Theory β) := ∃ V w, ⊧ᴹ[⟨F, V⟩, w] Γ
+def Theory.FrameSatisfiable (F : Frame α) (Γ : Theory β) := ∃ V w, w ⊩ᴹ[⟨F, V⟩] Γ
 
 def Theory.FrameClassSatisfiable (𝔽 : FrameClass α) (Γ : Theory β) := ∃ F ∈ 𝔽, Γ.FrameSatisfiable F
 
@@ -352,16 +425,24 @@ end AxiomDefinabilities
 
 section LogicDefinabilities
 
-variable [Inhabited α] [Inhabited β] (F: Frame α)
+variable [Inhabited α] [Inhabited β] {F: Frame α}
 
-attribute [simp] LogicKD LogicKT4
+def FrameClassDefinability (Λ : AxiomSet β) (P : Frame α → Prop) := ∀ {F : Frame α}, (P F) ↔ (F ∈ 𝔽(Λ))
 
-lemma LogicK.def_FrameClass : F ∈ 𝔽((𝐊 : AxiomSet β)) := by apply AxiomK.defines;
+instance LogicK.FrameClassDefinability : @FrameClassDefinability α β 𝐊 (λ _ => True) := by
+  intro F;
+  constructor;
+  . intros; apply AxiomK.defines;
+  . simp;
 
-instance : Nonempty (𝔽((𝐊 : AxiomSet β)) : FrameClass α) := ⟨(λ _ _ => True), (by apply LogicK.def_FrameClass)⟩
+instance : Nonempty (𝔽((𝐊 : AxiomSet β)) : FrameClass α) := by
+  existsi (λ _ _ => True);
+  apply LogicK.FrameClassDefinability.mp;
+  trivial;
 
-lemma LogicKD.def_FrameClass : (Serial F) ↔ F ∈ 𝔽((𝐊𝐃 : AxiomSet β)) := by
-  simp only [LogicKD, AxiomSetFrameClass.union];
+instance LogicKD.FrameClassDefinability : @FrameClassDefinability α β 𝐊𝐃 Serial := by
+  intro F;
+  simp [LogicKD, AxiomSetFrameClass.union, -AxiomSetFrameClass];
   constructor;
   . intro hSerial;
     have := (AxiomK.defines β F);
@@ -371,13 +452,14 @@ lemma LogicKD.def_FrameClass : (Serial F) ↔ F ∈ 𝔽((𝐊𝐃 : AxiomSet β
     apply (AxiomD.defines β F).mpr;
     simp_all;
 
-instance : Nonempty (𝔽((𝐊𝐃 : AxiomSet β)) : FrameClass α) := ⟨
-  (λ _ _ => True),
-  (by apply (LogicKD.def_FrameClass _).mp; simp [Serial];)
-⟩
+instance : Nonempty (𝔽((𝐊𝐃 : AxiomSet β)) : FrameClass α) := by
+  existsi (λ _ _ => True);
+  apply LogicKD.FrameClassDefinability.mp;
+  simp [Serial];
 
-lemma LogicS4.def_FrameClass : (Reflexive F ∧ Transitive F) ↔ (F ∈ 𝔽((𝐒𝟒 : AxiomSet β))) := by
-  simp only [LogicS4, LogicKT4, AxiomSetFrameClass.triunion];
+instance LogicS4.FrameClassDefinability : @FrameClassDefinability α β 𝐒𝟒 (λ F => (Reflexive F ∧ Transitive F)) := by
+  intro F;
+  simp [LogicKT4, AxiomSetFrameClass.triunion, -AxiomSetFrameClass];
   constructor;
   . rintro ⟨hRefl, hTrans⟩;
     have := (AxiomK.defines β F);
@@ -389,13 +471,14 @@ lemma LogicS4.def_FrameClass : (Reflexive F ∧ Transitive F) ↔ (F ∈ 𝔽((�
     . apply (AxiomT.defines β F).mpr; simp_all;
     . apply (Axiom4.defines β F).mpr; simp_all;
 
-instance : Nonempty (𝔽((𝐒𝟒 : AxiomSet β)) : FrameClass α) := ⟨
-  (λ _ _ => True),
-  (by apply (LogicS4.def_FrameClass _).mp; simp [Reflexive, Transitive];)
-⟩
+instance : Nonempty (𝔽((𝐒𝟒 : AxiomSet β)) : FrameClass α) := by
+  existsi (λ _ _ => True);
+  apply LogicS4.FrameClassDefinability.mp;
+  simp [Reflexive, Transitive];
 
-lemma LogicS5.def_FrameClass : (Reflexive F ∧ Euclidean F) ↔ F ∈ 𝔽((𝐒𝟓 : AxiomSet β)) := by
-  simp only [LogicS5, LogicKT5, AxiomSetFrameClass.triunion];
+instance LogicS5.FrameClassDefinability : @FrameClassDefinability α β 𝐒𝟓 (λ F => (Reflexive F ∧ Euclidean F)) := by
+  intro F;
+  simp [LogicKT5, AxiomSetFrameClass.triunion, -AxiomSetFrameClass];
   constructor;
   . rintro ⟨hRefl, hEucl⟩;
     have := (AxiomK.defines β F);
@@ -407,30 +490,10 @@ lemma LogicS5.def_FrameClass : (Reflexive F ∧ Euclidean F) ↔ F ∈ 𝔽((�
     . apply (AxiomT.defines β F).mpr; simp_all;
     . apply (Axiom5.defines β F).mpr; simp_all;
 
-instance : Nonempty (𝔽((𝐒𝟓 : AxiomSet β)) : FrameClass α) := ⟨
-  (λ _ _ => True),
-  (by apply (LogicS5.def_FrameClass _).mp; simp [Reflexive, Euclidean];)
-⟩
-
-/-
-lemma LogicGL.def_FrameClass : ∀ f, (Transitive f ∧ WellFounded f) ↔ (F ∈ FrameClass α β 𝐆𝐋) := by
-  simp only [LogicGL];
-  intro f;
-  constructor;
-  . intro hR;
-    apply Theory.frames_union.mpr ⟨
-      (AxiomK.defines β F),
-      (AxiomL.defines β F).mp hR
-    ⟩;
-  . intro hp;
-    apply (AxiomL.defines β F).mpr;
-    aesop;
-
-lemma LogicGL.trivialFrame : ∃ f, F ∈ FrameClass α β 𝐆𝐋 := by
+instance : Nonempty (𝔽((𝐒𝟓 : AxiomSet β)) : FrameClass α) := by
   existsi (λ _ _ => True);
-  apply (def_FrameClass _).mp;
-  simp [Transitive];
--/
+  apply LogicS5.FrameClassDefinability.mp;
+  simp [Reflexive, Euclidean]
 
 end LogicDefinabilities
 
